and aes128

code/experimental/aes/Hacl.AES_128.BitSlice.fst
@@ -72,6 +72,20 @@ val aes128_update4:
 
 let aes128_update4 out inp ctx ctr = aes_update4 out inp ctx ctr
 
+inline_for_extraction
+val aes128_ctr:
+  len: size_t
+  -> out: lbuffer uint8 len
+  -> inp: lbuffer uint8 len
+  -> ctx: aes_ctx
+  -> counter: size_t
+  -> ST unit
+  (requires (fun h -> live h out /\ live h inp /\ live h ctx))
+  (ensures (fun h0 _ h1 -> modifies (loc out) h0 h1))
+
+let aes128_ctr len out inp ctx c = aes_ctr #M32 #Spec.AES.AES128 len out inp ctx c
+
+
 [@ CInline ]
 val aes128_ctr_encrypt:
     len: size_t
